wip: distinguish between a concrete state having *any* abstract representation and it having a *valid* one, since validity can be broken within API calls

coq-verification/src/Concrete/MM/Proofs.v
@@ -18,12 +18,12 @@ Section Proofs.
   Context {ap : @abstract_state_parameters paddr_t nat}
           {cp : concrete_params}.
 
-  Local Definition preserves_represents
+  Local Definition preserves_represents_valid
         (f : concrete_state -> concrete_state) : Prop :=
     forall (conc : concrete_state),
-      (exists abst, represents abst conc) ->
-      exists abst', represents abst' (f conc).
-  Hint Unfold preserves_represents.
+      (exists abst, represents_valid abst conc) ->
+      exists abst', represents_valid abst' (f conc).
+  Hint Unfold preserves_represents_valid.
 
   Ltac simplify_step :=
     match goal with
@@ -36,9 +36,9 @@ Section Proofs.
     end.
   Ltac simplify := repeat simplify_step.
 
+  (* mm_free_page_pte doesn't change the state *)
   Lemma mm_free_page_pte_represents (conc : concrete_state) pte level ppool :
-    preserves_represents
-      (fun conc => fst (mm_free_page_pte conc pte level ppool)).
+    fst (mm_free_page_pte conc pte level ppool) = conc.
   Proof.
     autounfold.
     generalize dependent conc. generalize dependent pte.
@@ -50,90 +50,99 @@ Section Proofs.
              end.
   Qed.
 
+  (* mm_replace_entry doesn't change the state (it does in C, but in the Coq
+     translation it returns a new table to the caller and the caller updates the
+     state) *)
   Lemma mm_replace_entry_represents
         (conc : concrete_state)
         begin t pte_index new_pte level flags ppool :
-    preserves_represents
-      (fun conc =>
-         snd (fst (mm_replace_entry
-                     conc begin t pte_index new_pte level flags ppool))).
+    snd (fst (mm_replace_entry
+                conc begin t pte_index new_pte level flags ppool)) = conc.
   Proof.
     autounfold; cbv [mm_replace_entry].
     repeat match goal with
            | _ => simplify_step
-           | _ => apply mm_free_page_pte_represents
+           | _ => rewrite mm_free_page_pte_represents
            end.
   Qed.
 
+  (* mm_populate_table_pte doesn't change the state (it does in C, but in the Coq
+     translation it returns a new table to the caller and the caller updates the
+     state) *)
   Lemma mm_populate_table_pte_represents
         (conc : concrete_state)
         begin t pte_index level flags ppool :
-    preserves_represents
-      (fun conc =>
-         snd (fst (mm_populate_table_pte
-                     conc begin t pte_index level flags ppool))).
+    snd (fst (mm_populate_table_pte
+                conc begin t pte_index level flags ppool)) = conc.
   Proof.
     autounfold; cbv [mm_populate_table_pte].
     repeat match goal with
            | _ => simplify_step
-           | _ => apply mm_replace_entry_represents
+           | _ => rewrite mm_replace_entry_represents
            end.
   Qed.
 
+  (* mm_map_level doesn't change the state (it does in C, but in the Coq
+     translation it returns a new table to the caller and the caller updates the
+     state) *)
   Lemma mm_map_level_represents
         (conc : concrete_state)
         t begin end_ attrs table level flags ppool :
-    preserves_represents
-      (fun conc =>
-         snd (fst (mm_map_level
-                     conc t begin end_ attrs table level flags ppool))).
+    (snd (fst (mm_map_level
+                 conc t begin end_ attrs table level flags ppool))) = conc.
   Proof.
     autounfold; cbv [mm_map_level].
     repeat match goal with
            | _ => simplify_step
            | _ => apply while_loop_invariant; [ | solver ]
-           | _ => apply mm_free_page_pte_represents
-           | _ => apply mm_replace_entry_represents
-           | _ => apply mm_populate_table_pte_represents
+           | _ => rewrite mm_free_page_pte_represents
+           | _ => rewrite mm_replace_entry_represents
+           | _ => rewrite mm_populate_table_pte_represents
            end.
   Qed.
+
+  (* placeholder; later there will be actual expressions for the new abstract
+     states *)
+  Axiom TODO : @abstract_state paddr_t nat.
 
   Lemma mm_map_root_represents
         (conc : concrete_state)
         t begin end_ attrs root_level flags ppool :
-    preserves_represents
-      (fun conc =>
-         snd (fst (mm_map_root
-                     conc t begin end_ attrs root_level flags ppool))).
+    forall abst,
+      represents abst conc ->
+      represents TODO
+                 (snd (fst (mm_map_root
+                              conc t begin end_ attrs root_level flags ppool))).
   Admitted.
 
   Lemma mm_ptable_identity_update_represents
         (conc : concrete_state)
         t pa_begin pa_end attrs flags ppool :
-    preserves_represents
-      (fun conc =>
-         snd (fst (mm_ptable_identity_update
-                     conc t pa_begin pa_end attrs flags ppool))).
+    forall abst,
+      represents abst conc ->
+      represents TODO
+                 (snd (fst (mm_ptable_identity_update
+                              conc t pa_begin pa_end attrs flags ppool))).
   Admitted.
 
   Lemma mm_identity_map_represents
         (conc : concrete_state)
         begin end_ mode ppool :
-    preserves_represents
+    preserves_represents_valid
       (fun conc => snd (fst (mm_identity_map conc begin end_ mode ppool))).
   Admitted.
 
   Lemma mm_defrag_represents
         (conc : concrete_state)
         ppool :
-    preserves_represents
+    preserves_represents_valid
       (fun conc => fst (mm_defrag conc ppool)).
   Admitted.
 
   Lemma mm_unmap_represents
         (conc : concrete_state)
         begin end_ ppool :
-    preserves_represents
+    preserves_represents_valid
       (fun conc => snd (fst (mm_unmap conc begin end_ ppool))).
   Admitted.
 End Proofs.
